WIP

theories/Foundations.v
@@ -1,5 +1,5 @@
 (* SLOT, proofs about distributed systems design
-   Copyright (C) 2019-2024  k32
+   Copyright (C) 2019-2025  k32
 
    This program is free software: you can redistribute it and/or modify
    it under the terms of the GNU General Public License as published by
@@ -23,7 +23,8 @@ From Coq Require Import
   List
   Ensembles
   Relation_Definitions
-  RelationClasses.
+  RelationClasses
+  SetoidClass.
 
 Import ListNotations.
 
@@ -68,24 +69,71 @@ process scheduler.
 
 [future s Future] represents a valid state transition.
 
-*)
+*** State class is a setoid.
+
+ *)
+
+Locate "==>".
+Check respectful.
+
+Print Setoid.
+
+Print exist.
 
 Section transition_system.
   Context {State Label Result : Type}.
 
-  Inductive Future :=
-  | fut_cont : Label -> State -> Future
-  | fut_result : Result -> Future.
+  (* Definition prop_equiv a b (pred : State -> Prop) : *)
+  (*   a == b -> *)
+  (*   pred a <-> pred b. *)
+
+  (*   Check pointwise_relation. *)
+
+  (* Inductive Eq_prop : relation (State -> Prop) := *)
+  (* | eq_prop : forall (a b : State -> Prop), Eq_prop a b. *)
 
   Class TransitionSystem :=
-    { future : State -> Future -> Prop
+    { cont : Label -> State -> State -> Prop;
+
+      terminal : State -> Result -> Prop;
+
+      state_setoid :: Setoid State;
     }.
+
+  Print pointwise_relation.
+
+
+  Add Parametric Morphism `{TransitionSystem} (l : Label) : (cont l)
+  with signature (@equiv State state_setoid) ++> (iff) as cont_mor.
+
+
+      cont_covariant :: equiv ==> equiv
+
+      cont_equiv : forall label s1 s2 s1',
+        cont label s1 s1' ->
+        s1 == s2 ->
+        exists s2',
+          cont label s2 s2' /\ s1' == s2';
+
+      terminal_equiv : forall s1 s2 result,
+        s1 == s2 ->
+        terminal s1 result <-> terminal s2 result;
+    }.
+  (* This forms a category with two objects: `State' and `Result`, and
+     the following morphisms:
+
+     - Label: carrier for the class of identity morphisms
+       $id_{State}$
+     - terminal: a singleton morphism $Hom(State, Result)$
+   *)
 End transition_system.
 
 Global Arguments TransitionSystem (_ _ _) : clear implicits.
 
-Notation "A '~[' L ']~>' S" := (A (fut_cont L S)) (at level 20) : slot_scope.
-Notation "A '~>[' R ']'"  := (A (fut_result R)) (at level 20) : slot_scope.
+Notation "A '~[' L ']~>' B" := (cont L A B) (at level 20) :
+slot_scope. Notation "A '~>[' R ']'" := (terminal A R) (at level 20) :
+slot_scope. Notation "A '~>[]'" := (terminal A I) (at level 21) :
+slot_scope.
 
 (** ** Paths through the state space
 
@@ -102,655 +150,55 @@ executing a trace [te :: trace], transitioning the system from [s] to
 
 *)
 
-Section state_reachability.
-  Context `{HT : TransitionSystem}.
+Section state_reachability. Context `{HT : TransitionSystem}.
 
-  Inductive Trace : State -> State -> list Label -> Prop :=
-  | tr_nil : forall s,
-      Trace s s []
-  | tr_cons : forall s s' s'' label trace,
-      future s ~[label]~> s' ->
-      Trace s' s'' trace ->
-      Trace s s'' (label :: trace).
+  Inductive Trace : list Label -> State -> State -> Prop := | tr_nil :
+  forall s, Trace [] s s | tr_cons : forall s s' s'' label trace, s
+  ~[label]~> s' -> Trace trace s' s'' -> Trace (label :: trace) s s''.
+
+  Lemma trace_equiv trace s1 s1' s2 : Trace trace s1 s1' -> s1 == s2
+  -> exists s2', Trace trace s2 s2' /\ s1' == s2'. Proof. intros H1.
+  generalize dependent s2. induction H1 as [|s1 s1' s1'' label trace
+  Hs1' Hs1'']; intros. - exists s2; sauto. - destruct (cont_equiv
+  label s1 s2 s1' H Hs1') as [s2' [Hs2 Hs1's2']]. destruct (IHHs1''
+  s2' Hs1's2') as [s2'' [HS2''
+  Hs12'']].
+  exists s2''. split. + constructor 2 with (s' := s2'); assumption. + assumption. Qed.
 
   (** ** Hoare logic of traces
 
     [HoareTriple] is a type of judgments about trace execution,
     stating that if precondition [pre] holds for the initial state
     [s], and there is path [trace] through the state space leading to
-    state [s'], then postcondition [post] must hold for [s']. *)
-  Definition HoareTriple (precondition  : State -> Prop)
-                         (trace         : list Label)
-                         (postcondition : State -> Prop) :=
-    forall s s',
-      Trace s s' trace -> precondition s ->
-      postcondition s'.
+    state [s'], then postcondition [post] must hold for [s'].
+    *) Definition HoareTriple (precondition : State -> Prop) (trace : list Label) (postcondition : State -> Prop) := forall s s', Trace trace s s' -> precondition s -> postcondition s'.
 
   (** ** Hoare triple for terminal states
 
     [RHoareTriple] is a type of judgments about trace execution,
     stating that if precondition [pre] holds for the initial state
     [s], and [trace] leads to some terminal state with result
-    [result], then postcondition [post] must hold for [result]. *)
-  Definition RHoareTriple (precondition  : State -> Prop)
-                          (trace         : list Label)
-                          (postcondition : Result -> Prop) :=
-    let postcondition' s := exists2 result, future s ~>[ result ] & postcondition result
-    in HoareTriple precondition trace postcondition'.
-End state_reachability.
+    [result], then postcondition [post] must hold for [result].
+    *) Definition RHoareTriple (precondition : State -> Prop) (trace : list Label) (postcondition : Result -> Prop) := let postcondition' s := exists2 result, s~>[result] & postcondition result in HoareTriple precondition trace postcondition'. End state_reachability.
 
 Global Arguments Trace {_ _ _} (_).
 
-Notation "'{{' a '}}' t '{{' b '}}'" := (HoareTriple a t b) (at level 40) : slot_scope.
-Notation "'{{}}' t '{{' b '}}'" := (HoareTriple (const True) t b) (at level 39) : slot_scope.
 
-Notation "'{{' a '}}' t '{<' b '>}'" := (RHoareTriple a t b) (at level 40) : slot_scope.
-Notation "'{{}}' t '{<' b '>}'" := (RHoareTriple (const True) t b) (at level 39) : slot_scope.
+Notation "'{{' a '}}' t '{{' b '}}'" := (HoareTriple a t b) (at level 40) : slot_scope. Notation "'{{}}' t '{{' b '}}'" := (HoareTriple (const True) t b) (at level 39) : slot_scope.
+
+Notation "'{{' a '}}' t '{<' b '>}'" := (RHoareTriple a t b) (at level 40) : slot_scope. Notation "'{{}}' t '{<' b '>}'" := (RHoareTriple (const True) t b) (at level 39) : slot_scope.
 
 (** ** Invariants
 
-  [StateInvariant] is a type of judgments stating that if execution
-  of a trace starts in a state where property [prop] holds, then the
-  same property will hold for each intermediate state during
-  execution of the trace. In other words: [prop] is a subset of the
-  state space, and if the system starts off in this subset, it always
-  stays in it.
-*)
-Section state_invariant.
-  Context `{HT : TransitionSystem} (invariant : State -> Prop).
+  [StateInvariant] is a type of judgments stating that if execution of
+  a trace starts in a state where property [prop] holds, then the same
+  property will hold for each intermediate state during execution of
+  the trace. In other words: [prop] is a subset of the state space,
+  and if the system starts off in this subset, it always stays in it.
+  *) Section state_invariant. Context `{HT : TransitionSystem} (invariant : State -> Prop).
 
   Let invariant_future s f := future s f \/ invariant s.
 
-  Local Instance invTransSys : @TransitionSystem State Label Result :=
-    {
-      future := invariant_future
-    }.
+  Local Instance invTransSys : @TransitionSystem State Label Result := { future := invariant_future }.
 
-  Definition StateInvariant (trace : list Label) : Prop :=
-    forall s s',
-      Trace invTransSys s s' trace.
-End state_invariant.
-
-(** * Ensembles of traces
-
-    Trace ensembles play one of central roles in SLOT, because from
-    SLOT point of view any system is nothing but a collection
-    (ensemble) of event traces that it can produce. *)
-Section trace_ensembles.
-  Context `{HT : TransitionSystem}.
-
-  Definition TraceEnsemble := Ensemble (list Label).
-
-  (** Hoare logic of trace ensembles consists of a single rule: *)
-  Definition EHoareTriple (precondition  : State -> Prop)
-                          (ensemble      : TraceEnsemble)
-                          (postcondition : State -> Prop) :=
-    forall t, In ensemble t ->
-         {{ precondition }} t {{ postcondition }}.
-
-  (** Same, but for the results: *)
-  Definition ERHoareTriple (precondition  : State -> Prop)
-                           (ensemble      : TraceEnsemble)
-                           (postcondition : Result -> Prop) :=
-    forall t, In ensemble t ->
-              {{ precondition }} t {< postcondition >}.
-
-  Definition OccupiedTraceEnsemble (e : TraceEnsemble) : Prop :=
-    exists t s s',
-      e t -> Trace HT s s' t.
-
-  Definition FullyOccupiedTraceEnsemble (e : TraceEnsemble) : Prop :=
-    forall t,
-      e t -> exists s s', Trace HT s s' t.
-End trace_ensembles.
-
-Notation "'-{{' a '}}' e '{{' b '}}'" := (EHoareTriple a e b)(at level 40) : slot_scope.
-Notation "'-{{}}' e '{{' b '}}'" := (EHoareTriple (const True) e b)(at level 40) : slot_scope.
-
-Notation "'-{{' a '}}' e '{<' b '>}'" := (ERHoareTriple a e b)(at level 40) : slot_scope.
-Notation "'-{{}}' e '{<' b '>}'" := (ERHoareTriple (const True) e b)(at level 40) : slot_scope.
-
-Section commutativity.
-  Section defn.
-    Context `{TS : TransitionSystem}.
-
-    Definition labels_commute (l1 l2 : Label) : Prop :=
-      forall (s s' : State),
-        Trace TS s s' [l1; l2] <-> Trace TS s s' [l2; l1].
-
-    Global Instance events_commuteSymm : Symmetric labels_commute.
-    Proof.
-      intros a b Hab s s''.
-      unfold labels_commute in *. specialize (Hab s s'').
-      now symmetry in Hab.
-    Qed.
-  End defn.
-End commutativity.
-
-Section trace_properties.
-  Context `{TS : TransitionSystem}.
-
-  (** [trace_split] is an important observation that there is a point
-  in the state space for each intermediate step of the trace
-  execution: *)
-  Lemma trace_split : forall s s'' t1 t2,
-      Trace TS s s'' (t1 ++ t2) ->
-      exists s', Trace TS s s' t1 /\ Trace TS s' s'' t2.
-  Proof with sauto.
-    intros.
-    generalize dependent s.
-    induction t1; intros.
-    - exists s. split...
-    - simpl in H.
-      inversion_clear H.
-      specialize (IHt1 s' H1).
-      destruct IHt1.
-      exists x. split...
-  Qed.
-
-  (** [trace_concat] lemma demonstrates that traces can be composed: *)
-  Lemma trace_concat : forall s s' s'' t1 t2,
-      Trace TS s s' t1 ->
-      Trace TS s' s'' t2 ->
-      Trace TS s s'' (t1 ++ t2).
-  Proof with sauto.
-    intros.
-    generalize dependent s.
-    induction t1...
-  Qed.
-
-  Lemma trace_commutateive_permutation s s' t t' :
-    Trace TS s s' t ->
-    RestrictedPermutation labels_commute t t' ->
-    Trace TS s s' t'.
-  Proof with sauto.
-    intros Hls Hperm.
-    generalize dependent s.
-    induction Hperm; intros; try sauto.
-    - replace (a :: b :: l) with ([a; b] ++ l) in Hls by reflexivity.
-      replace (b :: a :: l) with ([b; a] ++ l) by reflexivity.
-      apply trace_split in Hls.
-      destruct Hls as [s_ [Hs_ Hs']].
-      apply H in Hs_.
-      apply trace_concat with (s' := s_)...
-  Qed.
-End trace_properties.
-
-Section trace_equivalence.
-  Context `{T : TransitionSystem} (e e' : @TraceEnsemble Label).
-
-  Definition sufficient_replacement :=
-    forall t s s', e t ->
-              Trace T s s' t ->
-              exists t', e' t' /\ Trace T s s' t'.
-
-  Definition sufficient_replacement_p :=
-    forall t, e t ->
-         exists t', e' t' /\ RestrictedPermutation labels_commute t t'.
-
-  Theorem ht_sufficient_replacement P Q :
-    sufficient_replacement ->
-    -{{P}} e' {{Q}} -> -{{P}} e {{Q}}.
-  Proof.
-    intros He2 Heht t Ht s s' Hls Hpre.
-    destruct (He2 t s s' Ht Hls) as [t' [Ht' Hls']].
-    eapply Heht; eauto.
-  Qed.
-
-  Lemma comm_perm_sufficient_replacement :
-    sufficient_replacement_p ->
-    sufficient_replacement.
-  Proof.
-    intros Hsrp t s s' Ht Hls.
-    destruct (Hsrp t Ht) as [t' [Ht' Hperm]].
-    eapply trace_commutateive_permutation in Hperm; eauto.
-  Qed.
-End trace_equivalence.
-
-(** * Product of transition systems *)
-Section trans_prod.
-  Context {Label S1 S2 R1 R2 : Type}
-    `{T1 : TransitionSystem S1 Label R1} `{T2 : TransitionSystem S2 Label R2}.
-
-  Let State : Type := S1 * S2.
-
-  Inductive TransProdResult :=
-  | tpr_l : forall (result_left : R1) (state_right  : S2), TransProdResult
-  | tpr_r : forall (state_left  : S1) (result_right : R2), TransProdResult.
-
-  Inductive TransProdFuture : State -> @Future State Label TransProdResult -> Prop :=
-  | tpf_cc : forall (label : Label) (s1 s1' : S1) (s2 s2' : S2),
-      future s1 ~[label]~> s1' ->
-      future s2 ~[label]~> s2' ->
-      TransProdFuture (s1, s2) ~[label]~> (s1', s2')
-  | tpf_rc : forall s1 s2 r,
-      future s1 ~>[r] ->
-      TransProdFuture (s1, s2) ~>[tpr_l r s2]
-  | tpf_cr : forall s1 s2 r,
-      future s2 ~>[r] ->
-      TransProdFuture (s1, s2) ~>[tpr_r s1 r].
-
-  Instance transProd : @TransitionSystem State Label TransProdResult :=
-    { future := TransProdFuture }.
-
-  Lemma transition_system_prod_comm (l1 : Label) (l2 : Label) :
-    @labels_commute _ _ _ T1 l1 l2 ->
-    @labels_commute _ _ _ T2 l1 l2 ->
-    @labels_commute _ _ _ transProd l1 l2.
-  Proof.
-    unfold labels_commute, transProd.
-    intros HT1 HT2 [s_l s_r] [s''_l s''_r].
-    specialize (HT1 s_l s''_l). specialize (HT2 s_r s''_r).
-    split; intros H.
-    { inversion H. clear H. inversion H5. clear H5. inversion H10. clear H10. subst.
-      destruct s' as [s'_l s'_r].
-      inversion_clear H4. inversion_clear H9.
-      destruct HT1 as [HT1 _]. destruct HT2 as [HT2 _].
-      assert (HT1p : Trace T1 s_l s''_l [l1; l2]) by sauto. specialize (HT1 HT1p). clear HT1p.
-      assert (HT2p : Trace T2 s_r s''_r [l1; l2] ) by sauto. specialize (HT2 HT2p). clear HT2p.
-      sauto.
-    }
-    { inversion H. clear H. inversion H5. clear H5. inversion H10. clear H10. subst.
-      destruct s' as [s'_l s'_r].
-      inversion_clear H4. inversion_clear H9.
-      destruct HT1 as [_ HT1]. destruct HT2 as [_ HT2].
-      assert (HT1p : Trace T1 s_l s''_l [l2; l1]) by sauto. specialize (HT1 HT1p). clear HT1p.
-      assert (HT2p : Trace T2 s_r s''_r [l2; l1]) by sauto. specialize (HT2 HT2p). clear HT2p.
-      sauto.
-    }
-  Qed.
-End trans_prod.
-
-Global Arguments transProd {_ _ _ _ _} (_ _).
-
-Infix "<*>" := (transProd) (at level 98) : slot_scope.
-
-(** * Sum of transition systems *)
-Section trans_sum.
-  Context {S1 L1 R1 S2 L2 R2} `{T1 : TransitionSystem S1 L1 R1} `{T2 : TransitionSystem S2 L2 R2}.
-
-  Let State : Type := S1 * S2.
-
-  Let Label : Type := L1 + L2.
-
-  Let Result : Type := R1 * R2.
-
-  Inductive TransSumFuture : State -> @Future State Label Result -> Prop :=
-  | tsf_rr : forall s1 s2 r1 r2,
-      future s1~>[r1] ->
-      future s2~>[r2] ->
-      TransSumFuture (s1, s2) ~>[(r1, r2)]
-  | tsf_l : forall s1 s1' s2 label,
-      future s1 ~[label]~> s1' ->
-      TransSumFuture (s1, s2) ~[inl label]~> (s1', s2)
-  | tsf_r : forall s1 s2 s2' label,
-      future s2 ~[label]~> s2' ->
-      TransSumFuture (s1, s2) ~[inr label]~> (s1, s2').
-
-  Instance transSum : @TransitionSystem State Label Result :=
-    { future := TransSumFuture }.
-
-  Lemma transition_system_sum_comm (l1 : L1) (l2 : L2) :
-    @labels_commute _ _ _ transSum (inl l1) (inr l2).
-  Proof.
-    unfold labels_commute. intros s s'.
-    split; sauto.
-  Qed.
-End trans_sum.
-
-Global Arguments transSum {_ _ _ _ _ _} (_ _).
-
-Infix "<+>" := (transSum) (at level 99) : slot_scope.
-
-From Coq Require Import
-  Decidable.
-
-(** ** Canonical Traces *)
-Section canonical_order.
-  Class CanonicalOrder {Label} (canon_rel : relation Label) :=
-    {
-      (* Non-strict total order: *)
-      canon_decidable a b : decidable (canon_rel a b);
-      canon_total a b : canon_rel a b \/ canon_rel b a;
-      canon_trans :: Transitive canon_rel;
-      (* Reflexivity is important for ordering of events produced by
-      the same process: *)
-      canon_reflexive :: Reflexive canon_rel;
-      canon_antisymmetric a b := canon_rel a b -> canon_rel b a -> a = b;
-    }.
-
-  Section comm.
-    Context `{T : TransitionSystem} `{Hcanon : CanonicalOrder Label} (commut_dec : forall a b, decidable (labels_commute a b)).
-
-    Definition can_follow (a b : Label) :=
-      (~labels_commute a b) \/ (canon_rel a b).
-
-    Definition can_follow_hd (label : Label) (trace : list Label) : Prop :=
-      match trace with
-      | [] => True
-      | head :: _ =>
-          can_follow label head
-      end.
-
-    Lemma canon_rel_asymm a b : ~canon_rel a b -> canon_rel b a.
-    Proof.
-      intros H.
-      destruct (canon_total b a); destruct (canon_total a b); firstorder.
-    Qed.
-
-    Lemma can_follow_dec a b : decidable (can_follow a b).
-    Proof.
-      unfold can_follow.
-      specialize (commut_dec a b) as Hdcomm.
-      specialize (canon_decidable a b) as Hdcanon.
-      apply dec_not in Hdcomm.
-      apply dec_or; assumption.
-    Qed.
-
-    Lemma can_follow_hd_dec a t : decidable (can_follow_hd a t).
-    Proof.
-      destruct t.
-      - simpl. apply dec_True.
-      - simpl. apply can_follow_dec.
-    Qed.
-
-    Inductive CanonicalTrace : State -> State -> list Label -> Prop :=
-    | canontr_nil : forall s,
-        CanonicalTrace s s []
-    | canontr_cons : forall s s' s'' label trace,
-        future s ~[label]~> s' ->
-        can_follow_hd label trace ->
-        CanonicalTrace s' s'' trace ->
-        CanonicalTrace s s'' (label :: trace).
-
-    Lemma can_follow_hd_eq {te t1 t2} (Hfoll : can_follow_hd te t1) (Hhd : hd_error t1 = hd_error t2) :
-      can_follow_hd te t2.
-    Proof.
-      intros.
-      unfold can_follow_hd in *.
-      destruct t1, t2; try reflexivity.
-      - exfalso. inversion Hhd.
-      - simpl in Hhd. injection Hhd as H. now subst.
-    Qed.
-
-    Fixpoint canon_trace_add s s' s'' label t (Hlabel : future s ~[label]~> s')
-                             (Ht : CanonicalTrace s' s'' t)
-                             (Hfoll : ~can_follow_hd label t) {struct Ht} :
-      exists t', CanonicalTrace s s'' t' /\
-                 RestrictedPermutation labels_commute (label :: t) t' /\
-                 (hd_error t = hd_error t').
-    Proof with sauto.
-      inversion Ht as [| A s_ B label' t' Hs_ Hfoll' Ht']; subst; clear Ht.
-      - exfalso. (* Hfoll cannot hold for an empty list *)
-        clear canon_trace_add.
-        unfold not, can_follow_hd in Hfoll.
-        contradiction.
-      - assert (Hl'lcanon : canon_rel label' label). {
-          clear canon_trace_add.
-          firstorder.
-        }
-        assert (Hlcomm : labels_commute label label'). {
-          clear canon_trace_add.
-          unfold can_follow_hd, can_follow in Hfoll.
-          destruct (commut_dec label label').
-          + assumption.
-          + firstorder.
-        }
-        (* Use label commutativity to derive an intermediate state on
-        the [label'; label] path: *)
-        assert (Hll' : Trace T s s_ [label; label']). {
-          constructor 2 with s'. assumption. constructor 2 with s_. assumption. constructor.
-        }
-        apply Hlcomm in Hll'.
-        inversion Hll'. inversion H4. inversion H10. subst.
-        (* Case analysis: can we attach [label] to [t']? *)
-        destruct (can_follow_hd_dec label t') as [Hfoll'' | Hfoll''].
-        + (* Yes, we can. Proof by construction: *)
-          exists (label' :: label :: t').
-          repeat split.
-          * constructor 2 with s'0...
-          * constructor. assumption.
-        + (* No, we cannot. Proof by induction *)
-          specialize (canon_trace_add s'0 s_ s'' label t' H9 Ht' Hfoll'').
-          destruct canon_trace_add as [t'' [Ht'' [Hcomm'' Hhd'']]].
-          exists (label' :: t'').
-          repeat split.
-          * constructor 2 with s'0; auto.
-            eapply can_follow_hd_eq; eauto.
-          * sauto.
-    Defined.
-
-    Fixpoint canon_trace_ (s s'' : State) (t : list Label) (Ht : Trace T s s'' t)
-          {struct Ht} :
-      exists t' : list Label, CanonicalTrace s s'' t' /\ RestrictedPermutation labels_commute t t'.
-    Proof with sauto.
-      destruct Ht.
-      - exists []...
-      - apply canon_trace_ in Ht. clear canon_trace_. destruct Ht as [t' [Ht' Hperm]].
-        destruct (can_follow_hd_dec label t').
-        + exists (label :: t')...
-        + eapply canon_trace_add in Ht'; eauto.
-          destruct Ht' as [t'' [Ht'' [Hperm'' Hhd]]].
-          exists t''...
-    Qed.
-
-    Theorem canonicalize_trace s s' :
-      sufficient_replacement_p (Trace T s s') (CanonicalTrace s s').
-    Proof.
-      intros t Ht.
-      now apply canon_trace_.
-    Qed.
-  End comm.
-End canonical_order.
-
-Require Import ZArith.
-Open Scope positive_scope.
-Require Import String.
-
-Definition PID : Type := positive * positive.
-
-Inductive ProgramReturn :=
-| normal
-| error : string -> ProgramReturn.
-
-CoInductive Program {Request : Type} {Reply : Request -> Type} : Type :=
-| p_dead : (* Program terminted *)
-    ProgramReturn -> Program
-| p_spawn : (* Spawn a new process *)
-    forall (new : Program)
-           (continuation : PID -> Program)
-         , Program
-| p_cont : (* Program is doing I/O *)
-    forall (pending_req : Request)
-           (continuation : Reply pending_req -> Program)
-         , Program.
-
-(* begin details *)
-Notation "'do' V '<-' I ; C" := (p_cont (I) (fun V => C))
-    (at level 100, C at next level, V name, right associativity) : slot_scope.
-
-Notation "'return' R" := (p_dead R)
-    (at level 100, right associativity) : slot_scope.
-
-Notation "'done' R" := (p_cont (R) (fun _ => p_dead I))
-    (at level 100, right associativity) : slot_scope.
-
-Notation "'call' V '<-' I ; C" := (I (fun V => C))
-    (at level 100, C at next level, V ident,
-     right associativity,
-      only parsing) : slot_scope.
-
-Notation "'spawn' V '<-' I ; C" := (p_spawn (I) (fun V => C))
-    (at level 100, C at next level, V ident,
-     right associativity) : slot_scope.
-(* end details *)
-
-(** * Input/output
-
- *)
-
-Section iodefs.
-  Record IOp (Request : Type) (Reply : Request -> Type) :=
-    mk_IOp {
-        iop_pid : PID;
-        iop_req : Request;
-        iop_rep : Reply iop_req;
-      }.
-
-  Class IOHandler {Request : Type} {Reply : Request -> Type} : Type :=
-    mkHandler
-      { h_state : Type;
-        h_state_transition : h_state -> IOp Request Reply -> h_state -> Prop;
-      }.
-
-  Global Instance ioHandlerTransitionSystem `(IOHandler) : @TransitionSystem h_state (IOp Request Reply) True :=
-    {
-      future s f :=
-        match f with
-        | fut_result _ => False
-        | fut_cont l s' => h_state_transition s l s'
-        end
-    }.
-End iodefs.
-
-Section trace.
-  Context `{IOHandler}.
-
-  Inductive TraceElem :=
-  | te_iop : IOp Request Reply -> TraceElem
-  | te_spawn : PID -> @Program Request Reply -> PID -> TraceElem
-  | te_exit : PID -> ProgramReturn -> TraceElem.
-End trace.
-
-(** * Generic scheduler *)
-Section gen_scheduler.
-  Context {State GlobalState Label : Type}
-    (step : GlobalState -> GlobalState -> State -> list State -> Label -> Prop).
-
-  Record SchedulerState :=
-    mkSchedState
-      { gen_sched_l : list State;
-        gen_sched_s : GlobalState;
-      }.
-
-  Inductive GenSchedStep : SchedulerState -> @Future SchedulerState Label () -> Prop :=
-  | gen_sched_empty : forall s,
-      GenSchedStep {| gen_sched_l := []; gen_sched_s := s |} ~>[ () ]
-  | gen_sched_skip : forall a s s' l l' te,
-      GenSchedStep {| gen_sched_l := l; gen_sched_s := s |} ~[ te ]~> {| gen_sched_l := l'; gen_sched_s := s' |} ->
-      GenSchedStep {| gen_sched_l := a :: l; gen_sched_s := s |} ~[ te ]~> {| gen_sched_l := a :: l'; gen_sched_s := s' |}
-  | gen_sched_apply : forall a a' s s' l te,
-      step s s' a a' te ->
-      GenSchedStep {| gen_sched_l := a :: l; gen_sched_s := s |} ~[ te ]~> {| gen_sched_l := a' ++ l; gen_sched_s := s' |}.
-End gen_scheduler.
-
-Section node_scheduler.
-  Context `{IOHandler}.
-  Context (node_id : positive).
-
-  Let Thread : Type := (positive * @Program Request Reply).
-
-  Section prop.
-    Context (next_pid : positive).
-
-    Inductive NodeSchedulerStep : positive -> Thread -> list Thread -> @TraceElem Request Reply -> Prop :=
-    | nsc_dead :
-      forall pid ret,
-        let te := te_exit (node_id, pid) ret in
-        NodeSchedulerStep
-          next_pid
-          (pid, p_dead ret)
-          []
-          te
-    | nsc_spawn :
-      forall pid new cont,
-        let new_pid := (node_id, next_pid) in
-        let te := te_spawn (node_id, pid) new new_pid in
-        NodeSchedulerStep
-          (Pos.succ next_pid)
-          (pid, p_spawn new cont)
-          [(pid, cont new_pid); (next_pid, new)]
-          te
-    | nsc_do_iop :
-      forall pid request reply cont,
-        let te := te_iop (mk_IOp _ _ (node_id, pid) request reply) in
-        NodeSchedulerStep
-          next_pid
-          (pid, p_cont request cont)
-          [(pid, cont reply)]
-          te.
-  End prop.
-
-  Check @SchedulerState.
-
-  Definition NodeSchedulerState : Type := @SchedulerState Thread positive.
-
-  Definition NodeScheduler := GenSchedStep NodeSchedulerStep.
-End node_scheduler.
-
-Section network_scheduler.
-  Context `{IOH : IOHandler}.
-
-  Definition Node : Type := positive * @NodeSchedulerState Request Reply.
-
-  Inductive NetSchedulerStep : () -> () -> Node -> list Node -> @TraceElem Request Reply -> Prop :=
-  | net_sched : forall ns ns' te,
-      NodeScheduler ns ~[te]~> ns' ->
-      NetSchedulerStep () () ns [ns'] te.
-
-
-  Inductive NetSchedulerStep : Node -> list Node -> () -> @TraceElem Request Reply -> Prop :=
-  | net_sched :
-    forall node ns ns' te,
-      NodeScheduler node ns ns' te ->
-      NetSchedulerStep (node, ns) [(node, ns')] () te.
-
-  Definition NetScheduler (s s' : list Node) (te : @TraceElem Request Reply) : Prop :=
-    GenSchedStep NetSchedulerStep s s' () te.
-End network_scheduler.
-
-(** * Concurrency
-
- *)
-(* Section interleaving. *)
-(*   Context {Event : Type}. *)
-
-(*   (** Set of all possible interleaving of two traces is a trace *) *)
-(* (*   ensemble. As we later prove in [interleaving_to_permutation], this *) *)
-(* (*   definition is dual to [RestrictedPermutation] of two traces. *) *)
-(*   Inductive Interleaving : list Event -> list Event -> Ensemble (list Event) := *)
-(*   | ilv_cons_l : forall te t1 t2 t, *)
-(*       Interleaving t1 t2 t -> *)
-(*       Interleaving (te :: t1) t2 (te :: t) *)
-(*   | ilv_cons_r : forall te t1 t2 t, *)
-(*       Interleaving t1 t2 t -> *)
-(*       Interleaving t1 (te :: t2) (te :: t) *)
-(*   | ilv_nil : Interleaving [] [] []. *)
-(* End interleaving. *)
-
-(* Section singleton_process. *)
-(*   (* Context {Gen State Event} `{StateSpace State (ProcessEvent Event)} `{Generator Event Gen}. *) *)
-
-(*   (* Record SingletonProcess := *) *)
-(*   (*   singleton_process { _ : Gen }. *) *)
-
-(*   Inductive SingletonStep : SingletonProcess -> option (SingletonProcess * (ProcessEvent Event)) -> Prop := *)
-(*   | wrs_nil : forall g, *)
-(*       g ~~>x -> *)
-(*       SingletonStep (singleton_process g) None *)
-(*   | wrp_cons : forall g g' evt, *)
-(*       g ~~> g' & evt -> *)
-(*       SingletonStep (singleton_process g) (Some (singleton_process g', 0 @ evt)). *)
-
-(*   Global Instance singletonGen : Generator (ProcessEvent Event) SingletonProcess := *)
-(*     { gen_step := SingletonStep }. *)
-
-(*   Lemma singleton_gen_comm : *)
-(*     generator_events_commute SingletonProcess. *)
-(*   Proof. *)
-(*     intros g g' g'' te1 te2 Hpids Hg Hg'. *)
-(*     exfalso. *)
-(*     inversion Hg; inversion Hg'; subst. *)
-(*     sauto. *)
-(*   Qed. *)
-(* End singleton_process. *)
+  Definition StateInvariant (trace : list Label) : Prop := forall s s', Trace invTransSys s s' trace. End state_invariant.
