theories/Scheduler.v
@@ -1,0 +1,279 @@
+From Coq Require Import
+  ZArith
+  List
+  String
+  SetoidClass.
+
+Import ListNotations.
+Open Scope positive_scope.
+
+From SLOT Require Import
+  Trace.
+
+From Hammer Require Import
+  Tactics.
+
+Definition PID := list positive.
+
+Inductive ProgramReturn :=
+| normal
+| error : string -> ProgramReturn.
+
+CoInductive Program {Request : Type} {Reply : Request -> Type} : Type :=
+| p_dead : (* Program terminted *)
+    ProgramReturn -> Program
+| p_spawn : (* Spawn a new process *)
+    forall (new : Program)
+           (continuation : PID -> Program)
+         , Program
+| p_cont : (* Program is doing I/O *)
+    forall (pending_req : Request)
+           (continuation : Reply pending_req -> Program)
+         , Program.
+
+(* begin details *)
+Notation "'do' V '<-' I ; C" := (p_cont (I) (fun V => C))
+    (at level 100, C at next level, V name, right associativity) : slot_scope.
+
+Notation "'return' R" := (p_dead R)
+    (at level 100, right associativity) : slot_scope.
+
+Notation "'done' R" := (p_cont (R) (fun _ => p_dead I))
+    (at level 100, right associativity) : slot_scope.
+
+Notation "'call' V '<-' I ; C" := (I (fun V => C))
+    (at level 100, C at next level, V ident,
+     right associativity) : slot_scope.
+
+Notation "'spawn' V '<-' I ; C" := (p_spawn (I) (fun V => C))
+    (at level 100, C at next level, V ident,
+     right associativity) : slot_scope.
+(* end details *)
+
+Section iodefs.
+  Record IOp (Request : Type) (Reply : Request -> Type) :=
+    mk_IOp {
+        iop_pid : PID;
+        iop_req : Request;
+        iop_rep : Reply iop_req;
+      }.
+
+  Class IOHandler {Request : Type} {Reply : Request -> Type} : Type :=
+    mkHandler
+      { h_state : Type;
+        h_state_transition : h_state -> IOp Request Reply -> h_state -> Prop;
+        h_state_setoid :: Setoid h_state;
+      }.
+
+  Global Instance ioHandlerTransitionSystem `(IOHandler) : @TransitionSystem h_state (IOp Request Reply) True :=
+    {
+      future s f :=
+        match f with
+        | fut_result _ => False
+        | fut_cont l s' => h_state_transition s l s'
+        end;
+      state_setoid := h_state_setoid
+    }.
+End iodefs.
+
+Section naive_scheduler.
+  (* Scheduler is simply a list of trace elements, together with their
+  futures, in order that represents future execution: *)
+  Context `{IOH : IOHandler}.
+  Let Prog := @Program Request Reply.
+
+  Inductive TraceEvent :=
+  | te_spawn : forall (pid : PID) (new_thread : Prog), TraceEvent
+  | te_exit : forall (pid : PID) (result : ProgramReturn), TraceEvent
+  | te_iop : IOp Request Reply -> TraceEvent.
+
+  Record Task :=
+    { pid : PID;
+      nextchild : positive;
+    }.
+
+  Inductive Task' : TraceEvent -> Task -> NewTasks -> Prop :=
+  | task'exit : forall pid result task,
+      Task'
+        (te_exit pid result)
+        task
+        newtasks₀
+  | task'spawn : forall pid nc cont new,
+      let newpid := pid ++ [nc] in
+      Task'
+        (te_spawn newpid new)
+        {| pid := pid; nextchild := nc; cont := cont |}
+        newtasks₂ {| pid := pid; nextchild := nc |} {| pid := newpid; nextchild := new |}.
+
+
+  | thread'exit : forall pid next result,
+      Thread'
+        {| pid := pid; nextchild := next; prog := p_dead result |}
+        (te_exit pid result)
+        []
+  | thread'spawn : forall pid next new cont,
+      let newpid := pid ++ [next] in
+      Thread'
+        {| pid := pid; nextchild := next; prog := p_spawn new cont |}
+        (te_spawn newpid new)
+        [{| pid := pid; nextchild := Pos.succ next; prog := cont newpid |};
+         {| pid := newpid; nextchild := 1; prog := new |}].
+
+  Inductive Scheduler := sched : list Thread -> Scheduler.
+
+  Inductive schedule : Thread -> list Thread -> list Thread -> Prop :=
+  | schedule₁ : forall t l,
+      schedule t l (t :: l)
+  | schedule₂ : forall t a l l',
+      schedule t l l' ->
+      schedule t (a :: l) l'.
+End naive_scheduler.
+(* Section trie. *)
+(*   Context `{IOH : IOHandler}. *)
+
+(*   Let Prog := @Program Request Reply. *)
+
+(*   Inductive TraceEvent := *)
+(*   | te_spawn : forall (pid : PID) (new_thread : Prog), TraceEvent *)
+(*   | te_exit : forall (pid : PID) (result : ProgramReturn), TraceEvent *)
+(*   | te_iop : IOp Request Reply -> TraceEvent. *)
+
+(*   Definition lift_pid (cid : positive) (te : TraceEvent) : TraceEvent := *)
+(*       match te with *)
+(*       | te_spawn pid new => *)
+(*           te_spawn (cid :: pid) new *)
+(*       | te_exit pid result => *)
+(*           te_exit (cid :: pid) result *)
+(*       | te_iop {| iop_pid := pid; iop_req := req; iop_rep := rep |} => *)
+(*           te_iop {| iop_pid := cid :: pid; iop_req := req; iop_rep := rep |} *)
+(*       end. *)
+
+(*   Inductive Scheduler := *)
+(*   | sched₀ : forall (parent : positive) (children : @Σ Scheduler TraceEvent), *)
+(*       Scheduler *)
+(*   | sched₁ : forall (parent : positive) (nextpid : positive) (this : Prog) (children : @Σ Scheduler TraceEvent), *)
+(*       Scheduler. *)
+
+(*   Check @future. *)
+(*   Check @Σfuture. *)
+
+(*   Inductive Scheduler' : Scheduler -> @Future Scheduler TraceEvent True -> Prop := *)
+(*   | sched'₀ : forall parent σ σ' te, *)
+(*       let TS := {| future := Scheduler' |} in *)
+(*       let TS' := {| future := @Σfuture _ _ _ TS |} in *)
+(*       @future _ _ _ TS' σ ~[te]~> σ' -> *)
+(*       Scheduler' (sched₀ parent σ) ~[lift_pid parent te]~> (sched₀ parent σ'). *)
+
+
+(* forall npid new cont σ, *)
+(*       sched (npid ( *)
+
+(*   Inductive TrieStep : TrieNode -> @Future TrieNode Label True -> Prop := *)
+(*   | tstep_current : forall node fut, *)
+(*       mutation node fut -> *)
+(*       TrieStep node fut. *)
+(*   | tstep_child : forall this cid child child' rest label, *)
+(*       TrieStep child ~[label]~> child' -> *)
+(*       TrieStep *)
+(*         (trie_node this ((cid, child) :: rest)) ~[lift cid label]~> *)
+(*         (trie_node this ((cid, child') :: rest)) *)
+(*   | tstep_next_child : forall this skip rest fut, *)
+(*       TrieStep (trie_node this rest) fut -> *)
+(*       TrieStep (trie_node this (skip :: rest)) fut *)
+(*   | tstep_rem_child : forall this cid dead rest fut, *)
+(*       TrieStep dead ~>[I] -> *)
+(*       TrieStep (trie_node this ((cid, dead) :: rest)) fut -> *)
+(*       TrieStep (trie_node this rest) fut. *)
+(* End trie. *)
+
+(* Section scheduler. *)
+(*   Context {Request : Type} {Reply : Request -> Type}. *)
+
+(*   Record SchedulerNodeS := *)
+(*     { nextchild : positive; *)
+(*       this_thread : option Prog *)
+(*     }. *)
+
+(*   Definition SchedulerS : Type := @TrieNode SchedulerNodeS. *)
+
+(*   Definition sched_node_step (s : SchedulerS) (fut : @Future SchedulerS TraceEvent True) : Prop := *)
+(*     match s with *)
+(*       trie_node {| nextchild := next; this_thread := prog |} children => *)
+(*         match prog with *)
+(*         | None => *)
+(*             match children with *)
+(*             | [] => *)
+(*                 fut = fut_result I *)
+(*             | _ => *)
+(*                 False *)
+(*             end *)
+(*         | Some prog => *)
+(*             match prog with *)
+(*             | p_dead ret => *)
+(*                 let te := te_exit [] ret in *)
+(*                 let this' := {| nextchild := next; this_thread := None |} in *)
+(*                 fut = fut_cont te (trie_node this' children) *)
+(*             | p_cont req cont => *)
+(*                 exists rep, *)
+(*                 let te := te_iop {| iop_pid := []; iop_req := req; iop_rep := rep |} in *)
+(*                 let this' := {| nextchild := next; this_thread := Some (cont rep) |} in *)
+(*                 fut = fut_cont te (trie_node this' children) *)
+(*             | p_spawn new cont => *)
+(*                 let pid := [next] in *)
+(*                 let te := te_spawn pid new in *)
+(*                 let this' := {| nextchild := Pos.succ next; this_thread := Some (cont pid) |} in *)
+(*                 let newchild := trie_node {| nextchild := 1; this_thread := Some new |} [] in *)
+(*                 let children' := (next, newchild) :: children in *)
+(*                 fut = fut_cont te (trie_node this' children') *)
+(*             end *)
+(*         end *)
+(*     end. *)
+
+(*   Definition lift_pid (cid : positive) (te : TraceEvent) : TraceEvent := *)
+(*       match te with *)
+(*       | te_spawn pid new => *)
+(*           te_spawn (cid :: pid) new *)
+(*       | te_exit pid result => *)
+(*           te_exit (cid :: pid) result *)
+(*       | te_iop {| iop_pid := pid; iop_req := req; iop_rep := rep |} => *)
+(*           te_iop {| iop_pid := cid :: pid; iop_req := req; iop_rep := rep |} *)
+(*       end. *)
+
+
+(*   Global Instance schedulerTS : @TransitionSystem SchedulerS TraceEvent True := *)
+(*     { *)
+(*       future := TrieStep sched_node_step lift_pid *)
+(*     }. *)
+(* End scheduler. *)
+
+(* Section scheduler_tests. *)
+(*   Let Req := positive. *)
+(*   Let Rep (_ : Req) := True. *)
+
+(*   Let complete := trie_node {| nextchild := 1; this_thread := None |} []. *)
+(*   Let sys1 := trie_node {| nextchild := 1; this_thread := Some (@p_dead _ Rep normal) |} []. *)
+
+(*   Ltac inv A := inversion A; subst; clear A. *)
+
+(*   Goal forall t, Trace _ sys1 (trie_node ) t -> *)
+(*                  t = [te_exit [] normal]. *)
+(*   Proof. *)
+(*     intros. *)
+(*     inv H. cbn in H0. inv H0. *)
+(*     2:{ inversion_clear H6. } *)
+(*     2:{ inversion_clear H4. } *)
+(*     inv H2. subst pid s'. *)
+(*     inv H1. *)
+(*     cbn in H. *)
+
+(*     inversion H3; subst. subst pid s0 s1 s2 s'. *)
+(*     inversion H1; subst. *)
+
+
+
+(*     inversion_clear H0. *)
+(*     - inversion_clear H. *)
+(*       subst pid s0 s1 s2. *)
+(*       inversion_clear H1. *)
+(*       + reflexivity. *)
+(*       + inversion_clear H. *)
