theories/SigmaTests.v
@@ -1,0 +1,96 @@
+From SLOT Require Import
+  Trace.
+
+From Coq Require Import
+  List
+  ZArith.
+Import ListNotations.
+
+Open Scope positive_scope.
+
+Inductive Command := | foo | bar.
+
+Inductive Label :=
+| spawn : positive -> Label
+| cmd : positive -> Command -> Label.
+
+Record State :=
+  { id : positive;
+    commands : list Command;
+  }.
+
+Inductive State' : State -> @Future State Label True -> Prop :=
+| State'₀ : forall i,
+    State' {| id := i; commands := [] |}~>[]
+| State'₁ : forall i c cmds,
+    State' {| id := i; commands := c :: cmds |} ~[cmd i c]~>
+           {| id := i; commands := cmds |}.
+
+Instance tsState : TransitionSystem State Label True := { future := State' }.
+
+From Hammer Require Import
+  Tactics.
+
+Ltac inv a := inversion a; subst; clear a.
+
+Section sys1.
+  Let sys1 := Σ₁ {| id := 1; commands := [] |} (spawn 1) Σø.
+
+  Goal forall (t : list Label),
+      Trace _ sys1 Σø t ->
+      t = [spawn 1].
+  Proof.
+    intros.
+    inv H. simpl in *. inv H0.
+    - inv H2. apply Σø' in H1. destruct H1. now rewrite H.
+    - inv H2.
+    - inv H2.
+  Qed.
+End sys1.
+
+Section sys2.
+  Let sys2 := Σ₁ {| id := 1; commands := [foo] |} (spawn 1) Σø.
+
+  Goal forall (t : list Label),
+      Trace _ sys2 Σø t ->
+      t = [spawn 1; cmd 1 foo].
+  Proof.
+    intros. subst sys2.
+    inv H. cbv in *. inv H0.
+    - exfalso. inv H2.
+    - inv H2. inv H1. inv H.
+      + apply Σø' in H0. destruct H0. now rewrite H.
+      + exfalso. inv H2.
+      + inv H2.
+    - inv H2.
+  Qed.
+End sys2.
+
+Section sys3.
+  Let sys3 := Σ₁ {| id := 1; commands := [] |} (spawn 1)
+                (Σ₁ {| id := 2; commands := [] |} (spawn 2) Σø).
+
+  Goal forall (t : list Label),
+      Trace _ sys3 Σø t ->
+      t = [spawn 1; spawn 2] \/ t = [spawn 2; spawn 1].
+  Proof.
+    intros.
+    inv H. cbv in *. inv H0.
+    - simpl in H2. clear H2. inv H1. inv H.
+      + left. inv H0.
+        * reflexivity.
+        * inv H.
+      + exfalso. inv H0. inv H; inv H2.
+      + exfalso. inv H2.
+    - exfalso. inv H2.
+    - inv H1. inv H0.
+      + inv H. inv H1. inv H2. now right.
+      + exfalso. clear H3. inv H2.
+        * inv H.
+          -- inv H1.
+          -- simpl in H2. inv H2.
+          -- inv H3. inv H2.
+        * inv H3.
+        * inv H3.
+  Qed.
+End sys3.
