theories/TransitionSystem.v
@@ -1,0 +1,175 @@
+From Coq Require Import
+  Program
+  List
+  Ensembles
+  Relation_Definitions
+  RelationClasses
+  SetoidClass
+  SetoidDec.
+
+Section exists_equiv.
+  Context {S : Type} `{Setoid S}.
+
+  Definition exists_equiv (prop : S -> Prop) (s : S) : Prop :=
+    exists (s' : S), prop s' /\ s == s'.
+End exists_equiv.
+
+Notation "'exists{' A == B } , C" := (exists_equiv (fun A => C) B) (at level 300, A name, B name, C at level 300, right associativity) : type_scope.
+
+Hint Unfold exists_equiv : slot.
+
+Section covariant_relation.
+  Context {State : Type} `{Setoid State} (R : relation State).
+
+  Definition rel_covariant :=
+    forall (s1 s2 s1' : State),
+      s1 == s2 ->
+      R s1 s1' ->
+      exists{s2' == s1'}, R s2 s2'.
+End covariant_relation.
+
+Section defn.
+  Context {State Arrow Result : Type}.
+
+  Class StrictTransitionSystem := {
+      ts_morph : Arrow -> relation State;
+      ts_terminal : State -> Result -> Prop;
+    }.
+
+  Class TransitionSystem `{StrictTransitionSystem} := {
+      ts_setoid :: Setoid State;
+      ts_morph_covariance : forall (a : Arrow), rel_covariant (ts_morph a);
+    }.
+
+  Definition compose `{StrictTransitionSystem} (a b : relation State) : relation State :=
+    fun s s'' =>
+      exists2 s', a s s' & b s' s''.
+End defn.
+
+Notation "A '~[' B ']~>' C" := (ts_morph B A C) (at level 20) : slot_scope.
+Infix "∘" := compose : slot_scope.
+
+Section leibniz_ts.
+  Context `{HSTS: StrictTransitionSystem}.
+
+  Program Instance leibnizTS : @TransitionSystem _ _ _ HSTS | 10 := {
+      ts_setoid := eq_setoid State;
+    }.
+  Next Obligation.
+    intros s s'1 s'2 Heq H. cbn in *. subst. now exists s'2.
+  Qed.
+End leibniz_ts.
+
+Open Scope slot_scope.
+
+Section props.
+  Context `{HTs: TransitionSystem}.
+
+  Theorem ts_compose_assoc (a b c : relation State) (s s' : State) :
+    (a ∘ (b ∘ c)) s s' <-> ((a ∘ b) ∘ c) s s'.
+    firstorder.
+  Qed.
+
+  Lemma compose_covariance (a b : relation State) (Hcov_a : rel_covariant a) (Hcov_b : rel_covariant b) :
+    rel_covariant (a ∘ b).
+  Proof.
+    intros s1 s2 s1'' Heq Hs1''.
+    destruct Hs1'' as [s1' Hs1' Hs1''].
+    specialize (Hcov_a s1 s2 s1' Heq Hs1').
+    destruct Hcov_a as [s2' [Hs2' Heq']].
+    specialize (Hcov_b s1' s2' s1'' Heq' Hs1'').
+    destruct Hcov_b as [s2'' [Hs2'' Heq'']].
+    exists s2''. split.
+    - econstructor; eauto.
+    - assumption.
+  Qed.
+
+  Definition commutative (a b : relation State) : Prop :=
+    forall s s',
+      (a ∘ b) s s' <-> (b ∘ a) s s'.
+
+  Definition setoid_commutative (a b : relation State) : Prop :=
+    forall s s1',
+      ((a ∘ b) s s1' -> exists{s2' == s1'}, (b ∘ a) s s2') /\
+      ((b ∘ a) s s1' -> exists{s2' == s1'}, (a ∘ b) s s2').
+End props.
+
+From Hammer Require Import
+  Tactics.
+
+Theorem eq_setoid_commutative `{HST : StrictTransitionSystem} :
+  forall a b,
+    commutative a b <-> @setoid_commutative _ _ _ HST leibnizTS a b.
+Proof.
+  split; unfold commutative, setoid_commutative.
+  - sauto.
+  - unfold compose, exists_equiv, equiv, ts_setoid, leibnizTS, eq_setoid.
+    intros H s s''. specialize (H s s'').
+    sauto.
+Qed.
+
+Import ListNotations.
+
+Section trace.
+  Context `{HTS: TransitionSystem}.
+
+  Inductive Trace : list Arrow -> State -> State -> Prop :=
+  | tr_nil : forall s,
+      Trace [] s s
+  | tr_cons : forall s s' s'' arrow trace,
+      s ~[arrow]~> s' ->
+      Trace trace s' s'' ->
+      Trace (arrow :: trace) s s''.
+
+  Fixpoint trace_via_compose (t : list Arrow) : relation State :=
+    match t with
+    | [] => eq
+    | (a :: t) => (ts_morph a) ∘ trace_via_compose t
+    end.
+
+  Lemma trace_is_compose_fold :
+    forall t s s',
+      Trace t s s' <-> trace_via_compose t s s'.
+  Proof with easy.
+    intros t s s''.
+    split.
+    - intros Ht. induction Ht.
+      + easy.
+      + simpl. unfold compose.
+        exists s'...
+    - generalize dependent s. induction t; intros s Ht; simpl in Ht.
+      + rewrite Ht. constructor.
+      + destruct Ht as [s' Hs' Hs''].
+        specialize (IHt s' Hs'').
+        constructor 2 with (s' := s')...
+  Qed.
+
+  Lemma trace_equiv_covariance :
+    forall t, rel_covariant (Trace t).
+  Proof.
+    intros t.
+    induction t; intros s1 s2 s1' Hs12 Hs1'.
+    - inversion Hs1'. subst.
+      exists s2. split.
+      + constructor.
+      + assumption.
+    - inversion Hs1'; subst.
+      eapply ts_morph_covariance in H2; eauto.
+      destruct H2 as [s2_ [Hs2_ Heq]].
+      specialize (IHt s' s2_ s1' Heq H5).
+      destruct IHt as [s2' [Hs2' Heq']].
+      exists s2'; split.
+      + econstructor; eauto.
+      + assumption.
+  Qed.
+
+  Lemma trace_via_compose_eqiuv_covariance :
+    forall t, rel_covariant (trace_via_compose t).
+  Proof.
+    intros t s s1 s2 s1' Ht.
+    rewrite <-trace_is_compose_fold in Ht.
+    eapply trace_equiv_covariance in Ht; eauto.
+    destruct Ht as [s2' [Hs2' Hs]]. exists s2'.
+    rewrite <-trace_is_compose_fold. easy.
+  Qed.
+End trace.
